#+TITLE:Exercise Sheet 1
#+AUTHOR: Isitha Subasinghe
* Evaluation strategies
*** Complete the evaluation steps for `fibLouis 4'.
#+BEGIN_SRC haskell
fibLouis :: Int -> Int
fibLouis 0 = 0
fibLouis 1 = 1
fibLouis n = fibLouis (n-1) + fibLouis (n -2)
fibLouis 4 =
    (fibLouis (4-1) + fibLouis (4-2)) =
    (fibLouis 3 + (fibLouis (4-2)) =
    (fibLouis 3 + fibLouis 2) =
    (((fibLouis (3-1) + fibLouis (3-2))
        + (fibLouis (2-1) + fibLouis (2-2))) =
     ...
     ((fibLouis 2 + fibLouis 1)  + (fibLouis 1 + fibLouis 0)) =
     ((fibLouis (2-1) + fibLouis (2-2)) + fibLouis 1) + (fibLouis 1 + fibLouis 0) =
     ((fibLouis 1 + fibLouis 0) + fibLouis 1) + (fibLouis 1 + fibLouis 0) =
     ((1 + 0) + 1) + (1 + 0) =
     (1 + 1) + 1 =
     2 + 1 =
     3
#+END_SRC

** Complete the evaluations for `fibEva 4'.
#+BEGIN_SRC haskell
fibEva :: Int -> Int
fibEva n = fst (aux n)
           where
             aux 0 = (0,1)
             aux n = next (aux (n - 1))
             next (a,b) = (b, a + b)
fibEva 4 =
  fst (aux 4) =
  fst (next (aux (4 - 1))) =
  fst (next (aux 3)) =
  fst (next (next (aux (3 - 1)))) =
  fst (next (next (aux 2))) =
  fst (next (next (next (aux (2 - 1))))) =
  fst (next (next (next (aux 1)))) =
  fst (next (next (next (next (aux (1-1)))))) =
  fst (next (next (next (next (aux 0))))) =
  fst (next (next (next (next (0,1))))) =
  fst (next (next (next (1, 0 + 1)))) =
  fst (next (next (next (1, 1)))) =
  fst (next (next (1, 1 + 1))) =
  fst (next (next (1, 2))) =
  fst (next (2, 1 + 2)) =
  fst (next (2, 3)) =
  fst (3, 2+3) =
  fst (3, 5) =
  3

#+END_SRC
* Natural Deduction
** Paranethesize the following formulas.
a) $\text{A} \vee \text{B} \rightarrow \text{C} \rightarrow \text{A} \wedge \text{C} \vee \text{B} \wedge \text{C}$

   $(\text{A} \vee \text{B}) \rightarrow (\text{C} \rightarrow ((\text{A} \wedge \text{C}) \vee (\text{B} \wedge \text{C})))$

b) $(\text{A} \rightarrow \text{B} \rightarrow \text{C}) \rightarrow \text{A} \wedge \text{B} \rightarrow \text{C}$

   $((\text{A} \rightarrow (\text{B} \rightarrow \text{C})))$

** Prove that the formulas above are tautologies in intuitionistic logic using natural deduction.
a) $(\text{A} \vee \text{B}) \rightarrow (\text{C} \rightarrow ((\text{A} \wedge \text{C}) \vee (\text{B} \wedge \text{C})))$
** We define
* Headache of the week
